no dec_triv

src/certigrad/reference.lean
@@ -17,8 +17,20 @@ open tactic
 meta def prove_refs_neq : tactic unit :=
 do applyc `pair_neq_of_neq₁,
    H ← intro `H,
-   [H'] ← injection H | failed,
-   done <|> contra_nats_eq H' <|> (do [H''] ← injection H' | failed, contra_nats_eq H'')
+   Hs ← injection H,
+   match Hs with
+   | [] := done
+   | [H'] := contra_nats_eq H' <|>
+             (do H''_ty ← mk_app `certigrad.label.label_eq_of_to_nat [H'],
+                 note `H'' none H''_ty,
+                 get_local `H'' >>= contra_nats_eq)
+   | (x::y::xs) := fail "injection produced multiple hyps"
+   end
+
+example : (ID.str label.W_encode, [5]) ≠ (ID.str label.batch_start, []) := by prove_refs_neq
+example : (ID.str label.W_encode, [5]) ≠ (ID.nat 5, [2, 3]) := by prove_refs_neq
+example : (ID.nat 100, [5]) ≠ (ID.nat 11, []) := by prove_refs_neq
+example : (ID.str label.W_encode, [5]) ≠ (ID.str label.batch_start, []) := by prove_refs_neq
 
 end tactics
 
